small ifexpr cleanups

Validator/Regex/Enter.lean
@@ -9,9 +9,11 @@ namespace Regex
 
 def enter (r: Regex σ): IfExpr σ (symbols r) := IfExpr.mk (extract r).2
 
+def enter_with_alloc (r: Regex σ) := (extract r).2
+
 namespace IfExpr
 
-#guard enter (Regex.or (Regex.symbol 'a') (Regex.symbol 'b'))
-  = IfExpr.expr 'a'
-      (IfExpr.expr 'b' (IfExpr.res  #v[true, true]) (IfExpr.res  #v[true, false]))
-      (IfExpr.expr 'b' (IfExpr.res  #v[false, true]) (IfExpr.res  #v[false, false]))
+#guard enter (Regex.or (Regex.symbol 'a') (Regex.symbol 'b')) =
+  IfExpr.expr 'a'
+    (IfExpr.expr 'b' (IfExpr.res  #v[true, true]) (IfExpr.res  #v[true, false]))
+    (IfExpr.expr 'b' (IfExpr.res  #v[false, true]) (IfExpr.res  #v[false, false]))
